Test/Eval.lean
@@ -2,15 +2,10 @@ import Nunchaku
 import Test.Eval.Sound
 import Test.Eval.Perf
 
--- TODO: Figure out where Subtype.elim_20 did not get killed
-#eval_nunchaku_sound_decl Array.size_uset
-
--- TODO: handle Std.Associative
-#eval_nunchaku_sound_decl List.foldr_assoc
-
 -- TODO: handle False.rec
 -- TODO: handle exists being used to build a dependent and
 -- TODO: handle casts
+
 
 -- TODO: Figure out where Sum.rec is coming from
 #eval_nunchaku_sound_decl Sum.map_inl
